March 21

axioms_coq.v
@@ -1,93 +1,118 @@
-Require Import List.
 Require Import Coq.Sets.Constructive_sets.
-Require Import Coq.Arith.EqNat.
-Require Import Coq.Relations.Relation_Definitions.
-Require Import Coq.Relations.Relation_Operators.
-Require Import Coq.Arith.Compare_dec.
-Require Import parametes_coq.
-Require Import config_coq.
+Require Import Definitions.
 Require Import oper_semantic_coq.
-Import Config.
-Import parameters.
 Import Operational_Semantics.
 
-Infix "∩" := Rel_Intersect (at level 10).
-Infix "∪" := Rel_Union (at level 0).
-
-(*****************DEFINITIONS******************)
-
-(*Well-Formedness of an Execution*)
-Parameter WF : Exec->Prop.
-(*Well-Formedness of an Execution is equal to: *)
-Definition WF1 (Ex:Exec) :  Prop := forall (a:Effect), (Ex-A a) ->  ~(Ex-hb a a).
-Definition WF2 (Ex:Exec) := forall (a b : Effect), (Ex-A a) -> (Ex-A b) -> (Ex-vis a b)-> (Ex-sameobj a b).
-Definition WF3 (Ex:Exec) := forall (a b c: Effect), (Ex-so a b)/\(Ex-so b c) -> (Ex-so a c ).
-Definition WF4 (Ex:Exec) := forall (a:Effect), (Ex-A a) -> (Ex-sameobj a a).
-Definition WF5 (Ex:Exec) := forall (a b : Effect),(Ex-A a) -> (Ex-A b) ->   (Ex-sameobj a b)-> (Ex-sameobj b a).
-Definition WF6 (Ex:Exec) := forall (a b c: Effect), (Ex-A a) -> (Ex-A b) ->(Ex-A c) -> (Ex-sameobj a b)/\(Ex-sameobj b c) -> (Ex-sameobj a c ).
-Definition WF7 (Ex:Exec) := forall (a b : Effect), (~(Ex-A a)) \/(~(Ex-A b))  -> ~(Ex-so a b) /\  ~(Ex-vis a b) /\  ~(Ex-sameobj a b).
 
 
-(*------------------------------------------------------------------------------------------------------------------------*)
-(******************AXIOMS******************)
-Axiom FW: forall (Ex:Exec), (WF1 Ex) ->(WF2 Ex) ->(WF3 Ex) ->(WF4 Ex) ->(WF5 Ex) ->(WF6 Ex)-> (WF7 Ex) ->(WF Ex). (*WF1 to WF6 result WF*)
-Axiom WFhelp: forall (Ex:Exec), (WF Ex)->(WF1 Ex)/\(WF2 Ex)/\(WF3 Ex)/\(WF4 Ex)/\(WF5 Ex)/\(WF6 Ex)/\(WF7 Ex). (*and vice versa*)
 
-Axiom Freshness: forall  (Θ:Store)(ex1 ex2:Exec) (opk:op_key) (eff:Effect) (r:ReplID),  (*new effect in reductions is fresh*)
-                   [Θ|-ex1, opk ~r~> ex2, eff] -> ~ (Θ r) eff.
-Axiom CorrectFreshness: forall  (Θ:Store)(ex1 ex2:Exec) (opk:op_key) (eff:Effect) (r:ReplID),  (*new effect in reductions is fresh*)
+
+
+(*---Well-Formedness of Executions *)
+Axiom FW: forall (Ex:Exec), (WF1 Ex) ->(WF2 Ex) ->(WF3 Ex) ->(WF4 Ex) ->(WF5 Ex) ->(WF6 Ex)-> (WF7 Ex) ->(WF Ex). 
+Axiom WFhelp: forall (Ex:Exec), (WF Ex)->(WF1 Ex)/\(WF2 Ex)/\(WF3 Ex)/\(WF4 Ex)/\(WF5 Ex)/\(WF6 Ex)/\(WF7 Ex).
+
+
+
+(*---Freshness of the Newly Generated Effect *)
+Axiom Freshness: forall (Θ:Store)(ex1 ex2:Exec) (opk:op_key)(eff:Effect)(r:ReplID),  
+                   [Θ|-ex1, opk ~r~> ex2, eff] -> forall r, (dom Θ r)-> ~ (Θ r) eff.
+Axiom CorrectFreshness: forall(Θ:Store)(ex1 ex2:Exec)(opk:op_key)(eff:Effect)(r:ReplID), 
                           [Θ|-ex1, opk ~r~> ex2, eff] -> ~ (ex1-A) eff.
 
 
-Axiom sameobj_refl : forall (Ex:Exec)(e:Effect), Ex-sameobj e e.
-Axiom so_trans: forall (Ex:Exec)(a b c: Effect), Ex-so a b -> Ex-so b c -> Ex-so a c.
+(*---The Definition of Equality of two Session Soups *)
+Axiom  Sess_Equal : forall (S S':SessSoup), S=S' <-> forall (I:Soup_Ing), (In Soup_Ing S I <-> In Soup_Ing S' I).
+
+
+(*---Trivial Facts About Relations*)
 Axiom sameobj_trans: forall (Ex:Exec)(a b c: Effect), Ex-sameobj a b -> Ex-sameobj b c -> Ex-sameobj a c.
-Axiom Sameobj_Def: forall  (Θ:Store) (Ex Ex':Exec)(opk:op_key) (η:Effect) (r:ReplID) (a b: Effect),  [Θ |- Ex, opk ~r~> Ex', η] -> Ex-A a -> Ex-A b -> Ex-sameobj a b.
+Axiom Sameobj_Def: forall  (Θ:Store) (Ex Ex':Exec)(opk:op_key) (η:Effect) (r:ReplID) (a b: Effect),
+                     [Θ |- Ex, opk ~r~> Ex', η] -> Ex-A a -> Ex-A b -> Ex-sameobj a b.
+Axiom SO_Seq_General : forall (Ex:Exec) (a b:Effect), (Ex-so a b) <-> (lt (seq a) (seq b)). 
 
 
 
-
-
-
-    
-(*Trivial Axioms*)
-Axiom SessionOrder : forall (Ex:Exec)(eff eff':Effect), Ex-so eff eff' -> ((eff.(sess) = eff'.(sess))/\ (  (eff.(seq))+1 <= (eff'.(seq)) )).
-Axiom Why_Coq : forall i:SeqNo, (i=i-1)\/(i=i+1) -> False.
-Axiom Relation_Dom : forall (Ex:Exec) (eff:Effect), (~Ex-A eff ) ->  (~Ex-so eff eff).
-Axiom Vis_Domain : forall (Ex:Exec)(a:Effect), ((Rel_dom Ex-vis a) -> (Ex-A a)).
-Axiom So_Domain : forall (Ex:Exec)(a:Effect), ((Rel_dom Ex-so a) -> (Ex-A a)).
+(*---Relating Domain of the Relations to the Universe of Effects*)
+Axiom So_Domain :      forall (Ex:Exec)(a:Effect), ((Rel_dom Ex-so a)      -> (Ex-A a)).
+Axiom Vis_Domain :     forall (Ex:Exec)(a:Effect), ((Rel_dom Ex-vis a)     -> (Ex-A a)).
+Axiom Hbo_Domain :     forall (Ex:Exec)(a:Effect), ((Rel_dom Ex-hbo a)     -> (Ex-A a)).
 Axiom Sameobj_Domain : forall (Ex:Exec)(a:Effect), ((Rel_dom Ex-sameobj a) -> (Ex-A a)).
-Axiom Hbo_Domain : forall (Ex:Exec)(a:Effect), ((Rel_dom Ex-hbo a) -> (Ex-A a)).
 
-
+(*---The Definition of Equality of Soup Ingredients*)
 Axiom Seq_Uniq : forall (i i': SeqNo)(s s': SessID)(σ σ' : session), (<<s , i , σ >>) = (<<s', i' , σ' >>) -> i=i'.
+
+
+(*--- So only relates effects from the same session*)
+Axiom SO_SameSession : forall (Ex:Exec)(eff eff':Effect), Ex-so eff eff' -> (eff.(sess) = eff'.(sess)).
+
+(*---Decidability of Membership of a Soup *)
 Axiom Soup_comp : forall (Ex:Exec)(eff:Effect), (Ex-A eff)\/(~ Ex-A eff).
-Axiom natSeq: forall ss:SeqNo, ~(ss+1 <= (ss-1)). 
 
 
-(*The new produced effect does not precede existing effects *)
-Axiom  SO_NewEff: forall (Θ: Store)(Ex Ex':Exec) (opk:op_key)(η:Effect)(r:ReplID),
-                                          [Θ|-Ex, opk ~r~> Ex', η] -> (forall a:Effect, Θ r a -> ~ Ex-so η a).
+(*---Claimed in the Paper *)
+(*3 equal statements to the acyclicity of hb*)
+Axiom PaperH8: forall (Ex:Exec)(eff:Effect), ~ (Ex-hb eff eff)-> ((~Ex-vis eff eff) /\ (~ Ex-so eff eff)).
 
+Axiom PaperH8II : forall (Ex:Exec)(eff eff': Effect), ~((Ex-vis eff eff')/\ (Ex-so eff' eff)).
 
-
-
-(*So holds if an effects precedes another*)
-
-Axiom SO_Seq_General : forall (Ex:Exec) (a b:Effect), (Ex-so a b) <-> (lt (seq a) (seq b)).
-Axiom  SO_Seq : forall (Ex:Exec)(a b c:Effect), Ex-so a b -> seq b = seq c - 1 -> Ex-so a c.
-Axiom SO_SeqII : forall (Ex:Exec)(a b :Effect), seq a = seq b -1  -> Ex-so a b.
-Axiom  SO_SeqIII : forall (Ex:Exec)(a b c:Effect), Ex-so a b -> Ex-so b c  -> Ex-so a c.
-
-
-(*Claimed in the paper:  3 equal statements to the acyclicity of hb*)
-Axiom PaperH8: forall (Ex:Exec)(eff:Effect),~ (Ex-hb eff eff)->
-                                     ~Ex-vis eff eff /\ ~ Ex-so eff eff  .
-Axiom PaperH8II : forall (Ex:Exec)(eff eff': Effect), 
-                                     ~((Ex-vis eff eff')/\ (Ex-so eff' eff)).
 Axiom PaperH8III : forall (Ex:Exec), 
-                                      (forall (eff:Effect), Ex-A eff -> ~ Ex-vis eff eff) ->
-                                      (forall (eff:Effect), Ex-A eff -> ~ Ex-so  eff eff) ->
-                                      (forall (eff eff':Effect),Ex-A eff -> Ex-A eff' ->  ~((Ex-vis eff eff')/\ (Ex-so eff' eff))) ->
-                                                                                                                              (forall (eff:Effect),~(Ex-hb eff eff)).
+                     (forall (eff:Effect), Ex-A eff -> ~ Ex-vis eff eff) ->
+                     (forall (eff:Effect), Ex-A eff -> ~ Ex-so  eff eff) ->
+                     (forall (eff eff':Effect),Ex-A eff -> Ex-A eff' ->  ~((Ex-vis eff eff')/\ (Ex-so eff' eff))) ->
+                     (forall (eff:Effect),~(Ex-hb eff eff)).
+
+
+
+
+
+(*************************************************************************************************************************)
+(*=============================These Were Axioms Before, But Now Are Replaced with Other Axioms and Are Trivially Proved *)
+
+Lemma  SO_NewEff: forall (Θ: Store)(Ex Ex':Exec) (opk:op_key)(η:Effect)(r:ReplID),
+                    [Θ|-Ex, opk ~r~> Ex', η] -> (forall a:Effect, Θ r a -> ~ Ex-so η a).
+Proof. intuition. apply CorrectFreshness in H. apply WF_Relation with (a:= η) (b:=a) in H1; destruct H1.
+       apply So_Domain in H1; auto.
+Qed.
+
+Require Import Omega.
+
+Lemma SessionOrder : forall (Ex:Exec)(eff eff':Effect), Ex-so eff eff' -> ((eff.(sess) = eff'.(sess))/\ ((eff.(seq))+1 <= (eff'.(seq)))).
+Proof.
+  intros Ex a b Hso. split.
+  apply SO_SameSession in Hso; auto. apply SO_Seq_General in Hso. intuition.
+Qed.
+
+Lemma  SO_Seq : forall (Ex:Exec)(a b c:Effect), Ex-so a b -> seq b = seq c - 1 -> Ex-so a c.
+Proof.
+  intros Ex a b c. intros Hso Heq. apply SO_Seq_General. apply SO_Seq_General in Hso. intuition.
+Qed.
+
+Lemma SO_SeqII' : forall (Ex:Exec)(a b :Effect), (seq b>0)->seq a = seq b -1  -> Ex-so a b.
+Proof.
+  intros. apply SO_Seq_General. omega.
+Qed.
+
+Require Import Omega.
+Lemma Eneq_nat_cont : forall i:SeqNo, (i>0)->(i=i-1)\/(i=i+1) -> False.
+Proof. intros. omega.
+Qed.
+
+Lemma natSeq: forall ss:SeqNo, ~(ss+1 <= (ss-1)).
+Proof.
+  intros. omega.
+Qed.
+
+Lemma  SO_SeqIII : forall (Ex:Exec)(a b c:Effect), Ex-so a b -> Ex-so b c  -> Ex-so a c.
+Proof.
+  intros.
+  apply SO_Seq_General. apply SO_Seq_General in H. apply SO_Seq_General in H0. omega.
+Qed.
+
+
+Lemma Relation_Dom : forall (Ex:Exec) (eff:Effect), (~Ex-A eff ) -> (~Ex-so eff eff).
+  Proof.
+    intuition. apply WF_Relation with (a:=eff)(b:=eff)(r:=Ex-so) in H0. destruct H0.
+    apply So_Domain in H1; auto.
+Qed.
 
