oper_semantic_coq.v
@@ -4,137 +4,82 @@ Require Import Coq.Arith.EqNat.
 Require Import Coq.Relations.Relation_Definitions.
 Require Import Coq.Relations.Relation_Operators.
 Require Import Coq.Arith.Compare_dec.
-Require Import parametes_coq.
-Require Import config_coq.
+Require Import Definitions.
 
 Module Operational_Semantics.
-Import Config.
-Import parameters.
-(*Specific Union for EFFVIS Rule*)
-
-Definition Rid_to_nat (r:ReplID): nat :=
-  match r with
-    |Rid_cons n => n
-  end.
+  (*Equality between two Ensemble*)
+  Definition Set_Equi (A:Type) (E1 E2: Ensemble A) : Prop :=
+    (Included A E1 E2)/\(Included A E2 E1).
   
+
+  (*==================================Auxiliary Reduction [OPER]==============================*)
   
-Definition F_Union (θ:Store)(r:ReplID)(η:Effect) (rcheck:ReplID) :  Exec_A :=
-  if (beq_nat (Rid_to_nat r)(Rid_to_nat rcheck)) then  (Union Effect (θ r) (Singleton Effect η)) else St_Dom_Error.
-
-Definition Store_Union (Θ:Store) (r:ReplID) (η:Effect) :=
-  Union (ReplID -> Exec_A) (Singleton (ReplID -> Exec_A) Θ) (Singleton (ReplID -> Exec_A)(F_Union Θ r η)).  
-  
-(*Return inverse of a relation in Effects*)
-Inductive rtrn_invs (rel:Relation) (n:Effect) : Ensemble Effect  :=
-first: forall m:Effect, (rel m n) -> (rtrn_invs rel n) m.
-(*Equality between two Ensemble*)
-Definition Set_Equi (A:Type) (E1 E2: Ensemble A) : Prop :=
-(Included A E1 E2)/\(Included A E2 E1).
-Inductive Exec : Type :=
-|E : Exec_A->  Relation -> Relation -> Relation -> Exec.
-Definition return_vis (Ex:Exec): Relation := 
-match Ex with 
-|(E AA rr1 rr2 rr3) => rr1
-end.
-Definition return_so (Ex:Exec): Relation := 
-match Ex with 
-|(E AA rr1 rr2 rr3) => rr2
-end.
-Definition return_samobj (Ex:Exec): Relation := 
-match Ex with 
-|(E AA rr1 rr2 rr3) => rr3
-end.
-Notation "Ex -vis" := (return_vis Ex) (at level 0).
-Notation "Ex -so" := (return_so Ex) (at level 0).
-Notation "Ex -sameobj" := (return_samobj Ex) (at level 0).
-(*The last three relations are parameters for each execution, but*)
-Definition Rel_Closure (r:Relation):= clos_trans Effect r.
-Definition Rel_Union (r1 r2 :Relation) (a b :Effect):Prop  :=  r1 a b \/ r2 a b.
-Definition Rel_Intersect (r1 r2 :Relation) (a b :Effect):Prop  :=  r1 a b /\ r2 a b.
-Definition return_A (Ex:Exec) := match Ex with
-|(E A vis so sameobj) => A
-end.
-Definition hb (Ex:Exec) : Relation :=
-Rel_Closure (Rel_Union Ex-vis Ex-so).
-Definition soo (Ex:Exec) : Relation := (Rel_Intersect Ex-so Ex-sameobj).
-Definition hbo (Ex: Exec) : Relation := (Rel_Closure (Rel_Union (soo Ex) (Ex-vis))).
-Notation "Ex -A" := (return_A Ex) ( at level 0).
-Notation "Ex -soo" := (soo Ex) (at level 0).
-Notation "Ex -hb" := (hb Ex) (at level 0).
-Notation "Ex -hbo" := (hbo Ex) (at level 0).
-
-Notation " A '∈' B " := (dom B A) (at level 80).
-
-(*op_key is a tuple of the form <s,i,op>. Each Effect has an op_key*)
-Inductive op_key : Type:=
-|op_key_cons: SessID->SeqNo->OperName -> op_key.
-Notation " '<' s , i , op '>' " := (op_key_cons s i op) (at level 0, op at level 20).
-
-(********************************************************************************************************************************)
-(*************************************************Auxiliary Reduction [OPER]************************************************)
-
-Reserved Notation "'['  Θ '|-' A , C '~' r '~>' B , n ']'" (at level 80,Θ at level 10).
-Inductive Aux_Reduct (Θ:Store) (r: ReplID) : Exec -> op_key -> Exec -> Effect -> Prop :=
-OPER :  forall   (A A': Exec_A) (v: Value) 
-                                (vis so sameobj vis' so' sameobj' : Relation) 
-                                (s:SessID)(i:SeqNo) (op:OperName) (η η': Effect),
-              r ∈ Θ ->
+  Reserved Notation "'['  Θ '|-' A , C '~' r '~>' B , n ']'" (at level 80,Θ at level 10).
+  Inductive Aux_Reduct (Θ:Store) (r: ReplID) : Exec -> op_key -> Exec -> Effect -> Prop :=
+    OPER :  forall   (A A': Exec_A) (v: Value) 
+                (vis so sameobj vis' so' sameobj' : Relation) 
+                (s:SessID)(i:SeqNo) (op:OperName) (η η': Effect),
+              r ∈ Θ -> 
               (Compute (Θ r) op)=v -> 
               η.(sess)=s /\ η.(seq)=i /\ η.(val)=v /\ η.(oper)=op  ->
               (forall eff, ((A eff) /\ eff.(sess)=s /\ eff.(seq) = i-1) <-> eff=η' ) ->
-               (forall eff,(A eff \/ eff=η )<->(A' eff)) ->
+              (forall eff,(A eff \/ eff=η )<->(A' eff)) ->
               (forall (eff eff':Effect), (vis' eff eff')<->((((Θ r) eff)/\eff'=η)\/((A eff/\ A eff')/\(vis eff eff')))) ->
               (forall (eff eff':Effect), (so' eff eff') <-> ((((so eff η') \/ (eff=η'))/\(eff'=η)) \/ (so eff eff'))) ->
-              (forall eff eff', A' eff-> A' eff'-> (sameobj' eff eff')) 
-
-                                                 ->[ Θ |- (E A vis so sameobj), <s,i,op>   ~r~>  (E A' vis' so' sameobj') ,η]
-where "'[' Θ |- A , C '~' r '~>' B , n ']'" := (Aux_Reduct Θ r A C B n).
-
-
-
+              (forall eff eff', A' eff-> A' eff'-> (sameobj' eff eff')) ->
+              (i>0) 
+              ->[ Θ |- (E A vis so sameobj), <s,i,op>   ~r~>  (E A' vis' so' sameobj') ,η]
+                 
+                 where "'[' Θ |- A , C '~' r '~>' B , n ']'" := (Aux_Reduct Θ r A C B n).
 
 
 
-(*Operational Semantics - Figure 8*)
-(*********************************************************************************************)
-
-Variable Error_opcls:op_cls. (*Default return value if the session is empty *)
-Reserved Notation "'[[' A , B , C '--' τ ',' n '-->' A' , B' , C' ']]'" (at level 0, n at level 200, τ at level 100).
-Inductive Progress (η:Effect)(τ:ConsCls) :  Exec->Store->SessSoup ->Exec -> Store -> SessSoup ->Prop :=     
-
-|EFFVIS: forall (Σ: SessSoup) ( Θ Θ' :Store) (Ex:Exec) (r:ReplID),
-                                                                      (In (Store) (Store_Union Θ r η)  Θ')->
-                                                                      (dom Θ' = dom Θ)-> (r∈ Θ) ->
-                                                                      (Included Effect (Union Effect (rtrn_invs Ex-vis η) (rtrn_invs Ex-so η)) (Θ r))->
-                                                                      (Ex-A η)->
-                                                                       ~((Θ r)η)                                                                          
-                                                                                ->[[Ex,Θ,Σ --τ,η-->  Ex ,Θ' ,Σ ]]
-
-|EC: forall  (Θ:Store)(Σ: SessSoup)(Ex Ex':Exec)(ss:SessID)(ii:SeqNo) 
-                             (opp:OperName)(r:ReplID) (oplist:session), 
-       (τ=ec) -> [Θ |- Ex, <ss,ii,opp> ~r~> Ex', η] ->
-                                                                                [[Ex,Θ,Σ ||| (mkSoup_Ing ss ii ((mkop_cls opp τ)::oplist))  --τ,η-->  Ex' ,Θ ,Σ ||| (mkSoup_Ing ss (ii+1) oplist ) ]]                 
 
 
-|CC: forall (Ex Ex':Exec) (Θ:Store)(Σ: SessSoup)(r:ReplID)
-                         (ss:SessID)(ii:SeqNo)(opp:OperName)(oplist:session),  
-                                                                                (τ=cc)->
-                                                                                (Included Effect (rtrn_invs Ex'-so η) (Θ r))->
-                                                                                ([ Θ |- Ex, <ss,ii,opp> ~r~> Ex', η]) 
-                                                                                ->[[Ex,Θ,Σ||| (mkSoup_Ing ss ii ((mkop_cls opp τ)::oplist)) --τ,η-->  Ex' ,Θ ,Σ|||(mkSoup_Ing ss (ii+1) oplist ) ]]
+  (*================================== Operational Semantics ==============================*)
+
+  Variable Error_opcls:op_cls. (*Default return value if the session is empty *)
+  
+  Reserved Notation "'[[' A , B , C '--' τ ',' n '-->' A' , B' , C' ']]'" (at level 0, n at level 200, τ at level 100).
+  
+  Inductive Progress (η:Effect)(τ:ConsCls) :  Exec->Store->SessSoup ->Exec -> Store -> SessSoup ->Prop :=     
+
+  |EFFVIS: forall (Σ: SessSoup) ( Θ Θ' :Store) (Ex:Exec) (r:ReplID),
+             (In (Store) (Store_Union Θ r η)  Θ')->
+             (dom Θ' = dom Θ)->
+             (r∈ Θ) ->
+             (Included Effect (Union Effect (rtrn_invs Ex-vis η) (rtrn_invs Ex-so η)) (Θ r))->
+             (Ex-A η)->
+             ~((Θ r)η)->                                                                         
+             [[Ex,Θ,Σ --τ,η-->  Ex ,Θ' ,Σ ]]
+
+               
+  |EC: forall  (Θ:Store)(Σ: SessSoup)(Ex Ex':Exec)(ss:SessID)(ii:SeqNo) 
+          (opp:OperName)(r:ReplID) (oplist:session), 
+         (τ=ec) -> [Θ |- Ex, <ss,ii,opp> ~r~> Ex', η] ->
+         [[Ex,Θ,Σ ||| (mkSoup_Ing ss ii ((mkop_cls opp τ)::oplist))  --τ,η-->  Ex' ,Θ ,Σ ||| (mkSoup_Ing ss (ii+1) oplist ) ]]                 
 
 
-|SC: forall (Ex Ex':Exec) (Θ Θ':Store)(Σ: SessSoup)(r:ReplID)
-                          (ss:SessID)(ii:SeqNo)(opp:OperName)(oplist:session),  
-                                                                                 (τ=sc)->
-                                                                                 ([Θ|-Ex, <ss,ii,opp> ~r~> Ex', η])->
-                                                                                 (Included Effect (Ex-A)(Θ r))->
-                                                                                 (Included ReplID (dom Θ) (dom Θ') /\ Included ReplID (dom Θ') (dom Θ)) ->
-                                                                                 forall r':ReplID, ((dom Θ') r') ->  
-                                                                                                (Set_Equi Effect (Θ' r') (Union Effect (Θ r')  (Singleton Effect η)))
-                                                                                ->[[Ex,Θ,Σ||| (mkSoup_Ing ss ii ((mkop_cls opp τ)::oplist)) --τ,η-->  Ex' ,Θ' ,Σ|||(mkSoup_Ing ss (ii+1) oplist ) ]]
+  |CC: forall (Ex Ex':Exec) (Θ:Store)(Σ: SessSoup)(r:ReplID)
+         (ss:SessID)(ii:SeqNo)(opp:OperName)(oplist:session),  
+         (τ=cc)->
+         (Included Effect (rtrn_invs Ex'-so η) (Θ r))->
+         ([ Θ |- Ex, <ss,ii,opp> ~r~> Ex', η]) 
+         ->[[Ex,Θ,Σ||| (mkSoup_Ing ss ii ((mkop_cls opp τ)::oplist)) --τ,η-->  Ex' ,Θ ,Σ|||(mkSoup_Ing ss (ii+1) oplist ) ]]
 
-where " '[['  E , Θ , Σ  '--' τ , η '-->'  F , T ,  S ']]' " := (Progress η τ E Θ Σ F T S).
+
+  |SC: forall (Ex Ex':Exec) (Θ Θ':Store)(Σ: SessSoup)(r:ReplID)
+         (ss:SessID)(ii:SeqNo)(opp:OperName)(oplist:session),  
+         (τ=sc)->
+         ([Θ|-Ex, <ss,ii,opp> ~r~> Ex', η])->
+         (Included Effect (Ex-A)(Θ r))->
+         (Included ReplID (dom Θ) (dom Θ') /\ Included ReplID (dom Θ') (dom Θ)) ->
+         (forall r':ReplID, ((dom Θ') r') ->  
+                       (Set_Equi Effect (Θ' r') (Union Effect (Θ r')  (Singleton Effect η)))) ->
+         ((forall (r':ReplID)(a:Effect), ((dom Θ') r') -> (Ex-A a) -> (Ex'-hbo a η) -> ((Θ' r') a))) 
+         ->[[Ex,Θ,Σ||| (mkSoup_Ing ss ii ((mkop_cls opp τ)::oplist)) --τ,η-->  Ex' ,Θ' ,Σ|||(mkSoup_Ing ss (ii+1) oplist ) ]]
+
+            where " '[['  E , Θ , Σ  '--' τ , η '-->'  F , T ,  S ']]' " := (Progress η τ E Θ Σ F T S).
 
 
 
