Definitions.v
@@ -1,0 +1,115 @@
+Require Import List.
+Require Import Coq.Sets.Constructive_sets.
+Require Import Coq.Arith.EqNat.
+Require Import Coq.Relations.Relation_Definitions.
+Require Import Coq.Relations.Relation_Operators.
+Require Import Coq.Arith.Compare_dec.
+Require Import Coq.Strings.String.
+
+
+(*=================================Basic Definitions*)
+Parameter SessID : Set.
+Parameter OperName : Set.
+Parameter Value : Set.
+Definition SeqNo := nat.
+Inductive ConsCls:Type := ec: ConsCls |cc: ConsCls |sc: ConsCls.
+Inductive op_cls :Type := mkop_cls: OperName -> ConsCls -> op_cls. 
+
+
+(*================================ Effects and Soups and Sessions*)
+
+Record  Effect : Set := mkEffect {name:string; sess : SessID; seq : SeqNo; oper : OperName; val:Value}.
+Definition Exec_A := (Ensemble Effect).
+Parameter Compute: Exec_A -> OperName -> Value. 
+Definition session := list op_cls.
+Inductive Soup_Ing : Type := |mkSoup_Ing : SessID -> SeqNo -> session -> Soup_Ing.
+Definition SessSoup := (Ensemble Soup_Ing).
+Inductive op_key : Type:= op_key_cons: SessID->SeqNo->OperName -> op_key.
+
+Notation " '<' s , i , op '>' " := (op_key_cons s i op) (at level 0, op at level 20).
+Notation " '<<' A ',' B ',' C  '>>'  " := (mkSoup_Ing A B C)(at level 10).
+Notation " S  '|||'  I " :=  ( Union Soup_Ing S  (Singleton Soup_Ing I) ) (at level 80).
+(*================================ Stores and Replicas *)  
+Inductive ReplID:Type := Rid_cons: nat -> ReplID.
+Definition Store := ReplID -> Exec_A.
+Parameter dom : Store -> (Ensemble ReplID).
+Parameter St_Dom_Error : Exec_A. 
+Notation " A '∈' B " := (dom B A) (at level 80).
+
+
+Definition Rid_to_nat (r:ReplID): nat :=
+  match r with
+    |Rid_cons n => n
+  end.
+
+Definition F_Union (θ:Store)(r:ReplID)(η:Effect) (rcheck:ReplID) :  Exec_A :=  
+  if (beq_nat (Rid_to_nat r)(Rid_to_nat rcheck))
+  then  (Union Effect (θ r) (Singleton Effect η)) else St_Dom_Error.
+
+Definition Store_Union (Θ:Store) (r:ReplID) (η:Effect) :=
+  Union (ReplID -> Exec_A) (Singleton (ReplID -> Exec_A) Θ) (Singleton (ReplID -> Exec_A)(F_Union Θ r η)).  
+
+Definition WF_union (S:SessSoup) (I:Soup_Ing): Prop := ~In Soup_Ing S I. 
+
+(*================================ Relations of Effects *)
+Definition Relation := relation Effect.
+Parameter  Rel_dom : Relation -> (Ensemble Effect). 
+Axiom WF_Relation : forall (r:Relation)(a b:Effect), r a b -> Rel_dom r a /\ Rel_dom r b.
+
+(*Inverse of a relation*)
+Inductive rtrn_invs (rel:Relation) (n:Effect) : Ensemble Effect  :=
+  first: forall m:Effect, (rel m n) -> (rtrn_invs rel n) m.
+
+Definition Rel_Closure (r:Relation):= clos_trans Effect r.
+Definition Rel_Union (r1 r2 :Relation) (a b :Effect):Prop  :=  r1 a b \/ r2 a b.
+Definition Rel_Intersect (r1 r2 :Relation) (a b :Effect):Prop  :=  r1 a b /\ r2 a b.
+
+Infix "∩" := Rel_Intersect (at level 40).
+Infix "∪" := Rel_Union (at level 50).
+(*================================ Executions *)
+Inductive Exec : Type :=
+|E : Exec_A->  Relation -> Relation -> Relation -> Exec.
+Definition return_vis (Ex:Exec): Relation := 
+  match Ex with 
+    |(E AA rr1 rr2 rr3) => rr1
+  end.
+Definition return_so (Ex:Exec): Relation := 
+  match Ex with 
+    |(E AA rr1 rr2 rr3) => rr2
+  end.
+Definition return_samobj (Ex:Exec): Relation := 
+  match Ex with 
+    |(E AA rr1 rr2 rr3) => rr3
+  end.
+Definition return_A (Ex:Exec) :=
+  match Ex with
+    |(E A vis so sameobj) => A
+  end.
+
+Definition hb (Ex:Exec) : Relation := Rel_Closure (Rel_Union (return_vis Ex) (return_so Ex)).
+Definition soo (Ex:Exec) : Relation := (Rel_Intersect (return_so Ex) (return_samobj Ex)).
+Definition hbo (Ex: Exec) : Relation := (Rel_Closure (Rel_Union (soo Ex) (return_vis Ex))).
+
+Notation "Ex -vis" := (return_vis Ex) (at level 0).
+Notation "Ex -so" := (return_so Ex) (at level 0).
+Notation "Ex -sameobj" := (return_samobj Ex) (at level 0).
+Notation "Ex -A" := (return_A Ex) ( at level 0).
+Notation "Ex -soo" := (soo Ex) (at level 0).
+Notation "Ex -hb" := (hb Ex) (at level 0).
+Notation "Ex -hbo" := (hbo Ex) (at level 0).
+
+
+
+(*================================ Well-Formedness of Executions *)
+(*!!! This should be changed to a clean inductive definition*)
+
+Parameter WF : Exec -> Prop.
+
+Definition WF1 (Ex:Exec) := forall (a:Effect),     (Ex-A a) -> ~(Ex-hb a a).
+Definition WF2 (Ex:Exec) := forall (a b:Effect),   (Ex-A a) -> (Ex-A b) -> (Ex-vis a b)-> (Ex-sameobj a b).
+Definition WF3 (Ex:Exec) := forall (a b c:Effect), (Ex-so a b)/\(Ex-so b c) -> (Ex-so a c).
+Definition WF4 (Ex:Exec) := forall (a:Effect),     (Ex-A a) -> (Ex-sameobj a a).
+Definition WF5 (Ex:Exec) := forall (a b:Effect),   (Ex-A a) -> (Ex-A b) ->(Ex-sameobj a b)-> (Ex-sameobj b a).
+Definition WF6 (Ex:Exec) := forall (a b c:Effect), (Ex-A a) -> (Ex-A b) ->(Ex-A c) -> (Ex-sameobj a b)/\(Ex-sameobj b c) -> (Ex-sameobj a c).
+Definition WF7 (Ex:Exec) := forall (a b : Effect), (~(Ex-A a))\/(~(Ex-A b)) -> ~(Ex-so a b) /\ ~(Ex-vis a b) /\  ~(Ex-sameobj a b).
+
