Theorem8.v
@@ -6,9 +6,7 @@ Require Import Coq.Relations.Relation_Definitions.
 Require Import Coq.Relations.Relation_Operators.
 Require Import Coq.Arith.Compare_dec.
 Require Import Coq.Program.Tactics.
-Require Import parametes_coq.
-Require Import config_coq.
-Import Config.
+Require Import Definitions.
 Require Import oper_semantic_coq.
 Require Import axioms_coq.
 Require Import theorems_coq.
@@ -19,35 +17,15 @@ Require Import lemma5.
 Require Import Theorem7_Lemma.
 Require Import Theorem7.
 Require Import Omega.
-Import parameters.
 Import Operational_Semantics.
+Require Import Theorem8_Lemmas.
 
 
-Lemma Theorem8_dom_help : forall η θ r,  dom (F_Union θ r η) = Singleton ReplID r.
-Proof.
-intros.
-compute. admit.
-Qed.
-
-
-Lemma Theorem8_nat_help : forall i:SeqNo, (i<>0) -> (lt (i-1) i).
-Proof.
-  intros.
-  destruct i. 
-  -compute in H. assert (0=0). reflexivity. intuition.
-  - omega.
-Qed.
-  
-Lemma  Theorem8_beq_help:  forall η θ r,  F_Union θ r η r = Union Effect ( θ r) (Singleton Effect η).
-  Proof. admit. Qed.
-
-  
 Theorem Theorem8: forall Σ Ex Ex' θ θ' η τ Ing1 Ing2 ss ii σσ op, 
                      (Ing1 = (mkSoup_Ing ss ii ((mkop_cls op τ)::σσ))) ->
                      (Ing2 = (mkSoup_Ing ss (ii+1) σσ)) ->
                      (WF_union Σ Ing1) -> (WF_union Σ Ing2) ->
                      [[Ex,θ,(Σ||| Ing1) --τ,η-->  Ex' ,θ' , (Σ|||Ing2)]] ->
-
                      WF Ex -> CausCons θ Ex -> CausCons θ' Ex'.
 Proof. intros  Σ Ex Ex' θ θ' η τ Ing1 Ing2 ss ii σσ op HIng1 HIng2. intros HWF_Union1 HWF_Union2.
        intros HProg HWF HCausCons.
@@ -65,7 +43,7 @@ Proof. intros  Σ Ex Ex' θ θ' η τ Ing1 Ing2 ss ii σσ op HIng1 HIng2. intro
 
 
          
-        +inversion H7. rewrite H7. rewrite<- H7 in H4. rewrite Theorem8_dom_help in H4. destruct H4.
+        +inversion H7. rewrite H7. rewrite<- H7 in H4. apply Theorem8_dom_help' in H4. subst r'.
          (*nice so far*)
          rewrite <- H8 in H5.
          rewrite Theorem8_beq_help in H5.
@@ -104,74 +82,71 @@ Proof. intros  Σ Ex Ex' θ θ' η τ Ing1 Ing2 ss ii σσ op HIng1 HIng2. intro
 
 
 
-       - unfold CausCons. intros; rename η0 into η'; rename r0 into r'. rename H6 into Hreduct.
-         clear HWF_Union1 HWF_Union2 H HProg H0. rename H4 into HBO'. 
-         inversion Hreduct. subst.
-         remember (E A vis so sameobj) as Ex.
-         assert (Ex-hbo a η'). {
-           apply HBO'_HBO with
-           (Ex:=Ex)(Ex':= (E A' vis' so' sameobj'))(s:=ss0)
-                   (i:=ii0)(op:=opp)(η:=η)(r:=r)(θ:=θ');auto.
-           intro. intuition. subst. specialize (H9 a). apply H9 in H1.
-           destruct H1. 
-           subst.
-           (*apply hbo accyclic*)
+       - unfold CausCons. intros; rename η0 into η'; rename r0 into r'; rename H6 into Hreduct;
+                          clear HWF_Union1 HWF_Union2 H HProg H0; rename H4 into HBO'; rename θ' into θ.
+         unfold CausCons in HCausCons.
 
-
-           
-           inversion HBO'; subst.
-           +SCase"single step".
-            inversion H.
-            *SSCase"from soo".
-             inversion H0 as [Hso' Hsameobj']; simpl in Hso'; simpl in Hsameobj'; clear H0.
-             apply t_step. simpl. unfold soo. left.  split.
-             (*1Proof of so*)
-             specialize (H14 a η'). apply H14 in Hso'.
-             inversion Hso'.
-             (*1.1 proof from  (so a η'0 \/ a = η'0) /\ η' = η*)
-             destruct H0. rewrite H4; clear H4.
-             inversion H0.
-             (*1.1.1 proof from  (so a η'0)*)
-             replace so with ((E A vis so sameobj)-so) in H4.
-             rewrite SO_Seq_General.
-             rewrite SO_Seq_General  in H4. specialize (H8 η'0).
-             assert (seq η'0 = seq η - 1). { assert (seq η'0 = ii0-1). intuition. rewrite H6. intuition. }
-             rewrite H6 in H4. omega. reflexivity.
-             (*1.1.2 proof from  (a = η'0)*)
-             apply SO_Seq_General. rewrite H4.
-             replace (seq η'0) with (ii0 - 1). replace (seq η) with ii0.
-             apply Theorem8_nat_help. (***!***) admit. (******!****)
-             intuition.  specialize (H8 η'0). intuition. 
-             (*1.2 proof from so: trivial*)
-             apply H0.
-
-             (*2proof of sameobj*)
-             apply Sameobj_Def with (Ex:= (E A vis so sameobj)) (Ex':=  (E A' vis' so' sameobj'))
-                                                                (opk :=  < ss0, ii0, opp >)
-                                                                (η:=η)(r:=r)(Θ:= θ'); simpl;auto.
-             apply WF_Relation with (a:=a)(b:=η')(r:=sameobj') in Hsameobj'.
-             destruct Hsameobj'. replace (sameobj') with ((E A' vis' so' sameobj')-sameobj) in H0;auto.
-             apply Sameobj_Domain in H0; simpl in H0.
-             replace (sameobj') with ((E A' vis' so' sameobj')-sameobj) in H4;auto.
-             apply Sameobj_Domain in H4; simpl in H4.
-(*here we need to prove that A a and A η'*)
-             specialize (H9 a).
-             apply H9 in H0. destruct H0; auto.
-             subst. intuition.
-             apply SO_NewEff with (Ex:= E A vis so sameobj) (Ex':=  E A' vis' so' sameobj')
-                                                                (opk :=  < ss0, ii0, opp >)
-                                                                (η:=η)(r:=r)(Θ:= θ')(a:=η') in Hreduct.
-             
-             
-         }
-
-
-
+         apply HBO'_HBO with
+           (Ex:=Ex)(Ex':= Ex')(s:=ss0)
+                   (i:=ii0)(op:=opp)(η:=η)(r:=r)(θ:=θ) in HBO';auto.
                                
          unfold CausCons in HCausCons. specialize (HCausCons r' a η').
          apply HCausCons; auto.
+         apply WF_Relation with (r:=Ex-hbo)(a:=a)(b:=η') in HBO'. destruct HBO'.
+         apply Hbo_Domain in H. apply H.
+         intro. apply Freshness with (r0:=r') in Hreduct; auto. subst. contradiction.
 
-       -unfold CausCons. intros; rename η0 into η'; rename r0 into r'.
-         assert (Ex-hbo a η'). admit.
+
+       - unfold CausCons. intros; rename η0 into η'; rename r0 into r'; rename H7 into Hreduct;
+                          clear HWF_Union1 HWF_Union2 H HProg H0; rename H5 into HBO'; rename θ' into θ.
+         unfold CausCons in HCausCons.
+
+         apply HBO'_HBO with
+           (Ex:=Ex)(Ex':= Ex')(s:=ss0)
+                   (i:=ii0)(op:=opp)(η:=η)(r:=r)(θ:=θ) in HBO';auto.
+                               
          unfold CausCons in HCausCons. specialize (HCausCons r' a η').
          apply HCausCons; auto.
+         apply WF_Relation with (r:=Ex-hbo)(a:=a)(b:=η') in HBO'. destruct HBO'.
+         apply Hbo_Domain in H. apply H.
+         intro. apply Freshness with (r0:=r') in Hreduct; auto. subst. contradiction.
+
+
+
+
+         -clear HProg H HWF_Union1 HWF_Union2 H0. rename H2 into Hreduct.
+          unfold CausCons. intros. rename r0 into r''. rename η0 into η''.
+          generalize dependent (H7 r'').
+          intro Hr''. assert ( r'' ∈ θ') as Hr'; auto. apply H7 in H0. inversion H0; clear H6.
+          compute in H5. specialize (H5 η''). apply H5 in H1. inversion H1; try (compute in H5); try(inversion H5); subst; try(rename  η'' into η); try(rename r'' into r').
+          +SCase"η'' in θ(r')".
+           assert (Ex-A a \/ a=η). { inversion Hreduct; subst. specialize (H16 a). intuition. }
+           destruct H8.
+           *specialize (HCausCons r' a η'').
+            assert (r' ∈ θ). apply H4;auto.
+            apply H0. apply Union_introl. apply HCausCons; auto.
+            apply HBO'_HBO with (r:=r) (Ex:=Ex)(η:=η)(i:=ii0)(s:=ss0)(op:=opp)(θ:=θ) in H2; auto.
+            intro; subst. apply Freshness with (r0:=r') in Hreduct;auto.
+           *generalize dependent (H7 r'). intro Hrθ. apply Hrθ in Hr'. inversion Hr'.
+            compute in H11. specialize (H11 a). apply H11. apply Union_intror. intuition.
+            
+          +SCase"η'' equal to η".
+           inversion H6; subst; rename η'' into η.
+           assert (Ex-A a \/ a=η). { inversion Hreduct; subst. specialize (H16 a). intuition. }
+                                  assert (a<>η) as Haη. {intro; subst.  apply Lemma5 in Hreduct; auto.
+                                                        apply HBO_HB in H2.
+                                                        assert (~(Ex')-hb η η). apply WFhelp in Hreduct.
+                                                        destruct Hreduct. apply H9; auto.
+                                                        contradiction.
+                                                       }
+            destruct H8.
+           *SSCase"Ex-A a".
+            apply H10; auto.
+            
+
+           *SSCase"a=η". contradiction.
+
+
+
+
+            Qed.
