Theorem8_Lemmas.v
@@ -1,0 +1,71 @@
+Require Import case_coq.
+Require Import List.
+Require Import Coq.Sets.Constructive_sets.
+Require Import Coq.Arith.EqNat.
+Require Import Coq.Relations.Relation_Definitions.
+Require Import Coq.Relations.Relation_Operators.
+Require Import Coq.Arith.Compare_dec.
+Require Import Coq.Program.Tactics.
+Require Import Definitions.
+Require Import oper_semantic_coq.
+Require Import axioms_coq.
+Require Import theorems_coq.
+Require Import contract_definition.
+Require Import contract_subs.
+Require Import contract_Eval.
+Require Import lemma5.
+Require Import Theorem7_Lemma.
+Require Import Theorem7.
+Require Import Omega.
+Import Operational_Semantics.
+
+
+Lemma rid_same_binder: forall (r:ReplID), (beq_nat (Rid_to_nat r)(Rid_to_nat r)) = true.
+Proof.
+  intro r.
+  induction r. simpl. induction n.
+  reflexivity. simpl. apply IHn.
+Qed.
+
+  
+Lemma  Theorem8_beq_help:  forall η θ r,  F_Union θ r η r = Union Effect ( θ r) (Singleton Effect η).
+Proof. intros. unfold F_Union.
+         rewrite rid_same_binder. reflexivity.
+Qed.
+
+Axiom error_not_domain: forall (r:ReplID)(t:Store),  (t r = St_Dom_Error) <-> (~(dom t) r).
+Axiom ReplID_Equality_Decidable: forall (r r':ReplID), (r=r') \/ (r<>r').
+
+Lemma Theorem8_dom_help'_help: forall r r', r=r' <->  (beq_nat (Rid_to_nat r) (Rid_to_nat r')=true).
+Proof.
+  intros r r'.
+  split; intro H.
+  -Case"->".
+   rewrite <- H.
+   induction r. simpl. symmetry. apply beq_nat_refl.
+  -Case"<-". destruct r. destruct r' as [n']. simpl in H.
+   apply beq_nat_true  in H. rewrite H. reflexivity.
+Qed.   
+
+
+                                 
+Lemma Theorem8_dom_help' : forall η θ r' r,  dom (F_Union θ r η) r' -> r'=r.
+Proof.
+intros. 
+assert (r=r' \/ r<>r') as HRidDec; try( apply ReplID_Equality_Decidable).
+destruct HRidDec; auto. apply error_not_domain in H; intuition. 
+destruct (beq_nat (Rid_to_nat r) (Rid_to_nat r')) eqn:E. compute. apply Theorem8_dom_help'_help in E; intuition.
+unfold F_Union. rewrite E. reflexivity.
+Qed.
+
+
+  
+
+Lemma Theorem8_nat_help : forall i:SeqNo, (i<>0) -> (lt (i-1) i).
+Proof.
+  intros.
+  destruct i. 
+  -compute in H. assert (0=0). reflexivity. intuition.
+  - omega.
+Qed.
+
