theorems_coq.v
@@ -4,14 +4,16 @@ Require Import Coq.Arith.EqNat.
 Require Import Coq.Relations.Relation_Definitions.
 Require Import Coq.Relations.Relation_Operators.
 Require Import Coq.Arith.Compare_dec.
-Require Import parametes_coq.
-Require Import config_coq.
+Require Import Definitions.
 Require Import oper_semantic_coq.
 Require Import axioms_coq.
 Require Import Cases.
-Import Config.
-Import parameters.
 Import Operational_Semantics.
+
+
+
+
+
 
 (*********************************************************************************************************)
 (*Lemma if Ex is well formeed, vis and so and hb are acyclic*)
@@ -43,11 +45,12 @@ Lemma Vis'_Acyclicity :  forall (Θ: Store)(Ex Ex':Exec) (opk:op_key)(η:Effect)
 Proof.
     intros Θ Ex Ex' key η r; intros WF_H reduct_H. 
     apply WellFormed_res1 in WF_H. inversion WF_H; clear H0  WF_H.
-    inversion reduct_H.
+    inversion reduct_H. rename H8 into Hi; rename H9 into H8; rename H10 into H9; rename H11 into H10;
+    rename H12 into H11.
     unfold return_A. unfold return_vis. 
     intros a H_a. unfold not. intros vis'_H.
     specialize (H5 a a). apply H5 in vis'_H. inversion  vis'_H. 
-    -Case "Θ r a /\ a = η ". { inversion H12. rewrite H14 in H13. apply Freshness in reduct_H. contradiction reduct_H. }
+    -Case "Θ r a /\ a = η ". { inversion H12. rewrite H14 in H13. apply Freshness with (r0:=r) in reduct_H. contradiction reduct_H. apply H0. }
     -Case "(A a /\ A a) /\ vis a a". {specialize (H a). rewrite <- H8 in H. unfold return_A in H. unfold return_vis in H. 
                                                    inversion H12. inversion H13. apply H in H15. contradiction. }
 Qed.
@@ -62,7 +65,8 @@ Lemma So'_Acyclicity :  forall (Θ: Store)(Ex Ex':Exec) (opk:op_key)(η:Effect)(
 Proof. 
     intros Θ Ex Ex' key η r; intros WF_H reduct_H. 
     apply WellFormed_res1 in WF_H. inversion WF_H; inversion H0; clear H0 H H2  WF_H.
-    inversion reduct_H.
+    inversion reduct_H. rename H8 into Hi; rename H9 into H8; rename H10 into H9; rename H11 into H10;
+    rename H12 into H11.
     unfold return_A. unfold return_so. 
     intros a H_a. unfold not. intros so'_H. 
     specialize (H6 a a). apply H6 in so'_H. inversion so'_H.
@@ -79,9 +83,7 @@ Proof.
                                                assert (seq η = i-1). specialize (H3 η). intuition.
                                                assert (seq η = i). intuition.
                                                rewrite H17 in H16.
-                                               assert (forall i:SeqNo, i=i-1\/i=i+1 -> False).
-                                               apply Why_Coq. specialize (H18 i).
-                                               apply H18. left. apply H16. }
+                                               apply  Eneq_nat_cont with (i:=i); auto. }
    -Case "so a a". { assert (Ex-A a \/ ~Ex-A a). apply Soup_comp. inversion H13.
                 +SCase"Ex-A a". specialize (H1 a). apply H1 in H14. rewrite <- H8 in H14; unfold return_so in H14. contradiction.
                 +SCase"~(Ex-A a)". apply Relation_Dom in H14. rewrite <- H8 in H14; unfold return_so in H14. contradiction. }
@@ -98,20 +100,22 @@ Lemma hb'_Acyclicity: forall (Θ: Store)(Ex Ex':Exec) (s:SessID) (i:SeqNo)(op:Op
 Proof.
   intros Θ Ex Ex' s i op η r. intros H_reduct H_WF.
   (*Inversion on the reduction*)
-  inversion H_reduct.
-  clear H10 H1 H0 H H3 H6 s0 i0 op0 η0. rename H4 into  H_η; rename H5 into  H_η'; rename H8 into H_vis';
-  rename H11 into H_so';rename H12 into H_sameobj';rename H7 into H_Exec; rename H9 into H_Exec'.
+  inversion H_reduct.  subst. rename H13 into Hi.
+  rename H4 into  H_η; rename H5 into  H_η'; rename H7 into H_vis';
+  rename H9 into H_so';rename H12 into H_sameobj'.
+  remember (E A' vis' so' sameobj') as Ex'.  remember (E A vis so sameobj) as Ex.
+  rename HeqEx into H_Exec. rename HeqEx' into H_Exec'.
 
 
   (*************************************************Assertions that will be needed*)
   
   (*Trivial assertions*)
-  assert ((Ex')-A = A')    as H_EX'A.      rewrite <- H_Exec'; auto.
-  assert ((Ex')-vis = vis')as H_EX'vis.    rewrite <- H_Exec'; auto. 
-  assert ((Ex')-so = so')  as H_EX'so.     rewrite <- H_Exec'; auto.
-  assert ((Ex)-A = A)      as H_EXA.       rewrite <- H_Exec;  auto.
-  assert ((Ex)-vis = vis)  as H_EXvis.     rewrite <- H_Exec;  auto. 
-  assert ((Ex)-so = so)    as H_EXso.      rewrite <- H_Exec;  auto.
+  assert ((Ex')-A = A')    as H_EX'A.      rewrite  H_Exec'; auto.
+  assert ((Ex')-vis = vis')as H_EX'vis.    rewrite  H_Exec'; auto. 
+  assert ((Ex')-so = so')  as H_EX'so.     rewrite  H_Exec'; auto.
+  assert ((Ex)-A = A)      as H_EXA.       rewrite  H_Exec;  auto.
+  assert ((Ex)-vis = vis)  as H_EXvis.     rewrite  H_Exec;  auto. 
+  assert ((Ex)-so = so)    as H_EXso.      rewrite  H_Exec;  auto.
   assert (seq η' =  i - 1) as H_η'def.     specialize (H_η'  η'). intuition.
 
   (*ignore this->*)rename H_WF into temp; assert (WF Ex) as H_WF. exact temp.
@@ -128,7 +132,7 @@ Proof.
   assert (forall (Ex:Exec)(a b c:Effect), (Ex-so a b)->(seq b)=(seq c)-1 ->(Ex-so a c)) as H_soRefl. apply SO_Seq.
 
   (*Assert if b's sequence number is plus one of a's, the (so a b) holds.*)
-  assert (forall (Ex:Exec)(a b :Effect), seq a = seq b -1  -> Ex-so a b) as H_soDef. apply SO_SeqII.
+  assert (forall (Ex:Exec)(a b :Effect),(seq b>0)-> seq a = seq b -1  -> Ex-so a b) as H_soDef. apply SO_SeqII';auto.
 
   (*Claim from the Paper, H16 of the paper*)
   assert ((forall a:Effect,(Ex)-A a -> ~(Ex) -hb a a)-> (forall x y:Effect, ~(Ex-vis x y /\ Ex-so y x ))) as H16.
@@ -163,28 +167,28 @@ Proof.
             intuition.
             
             +SCase"(Θ r a)/\b=η AND (so b η')/\a=η".
-                     apply Freshness in H_reduct. rewrite H8 in H0. contradiction.
+                     apply Freshness with (r0:=r) in H_reduct; auto. rewrite H9 in H0. contradiction.
 
             +SCase"(Θ r a)/\b=η AND b=η'/\a=η".
-                     apply Freshness in H_reduct. rewrite H8 in H0. contradiction.
+                     apply Freshness with (r0:=r) in H_reduct; auto. rewrite H9 in H0. contradiction.
 
             +SCase"(Θ r a)/\b=η AND(so b a)".
-                     rewrite H7 in H5. specialize (H_newEff Θ Ex Ex' <s,i,op> η r).
-                     intuition; rename H8 into H_newEff.
+                     rewrite H8 in H5. specialize (H_newEff Θ Ex Ex' <s,i,op> η r).
+                     intuition; rename H9 into H_newEff.
                      specialize (H_newEff a ). rewrite  H_EXso in H_newEff.
                      auto.
 
             +SCase" (A a/\A b)/\(vis a b) AND a=η/\(so b η')".
                      specialize(H_soRefl Ex b η' η).
                      rewrite H_EXso in H_soRefl; rewrite H4 in H_soRefl; rewrite H_η'def in H_soRefl.
-                     intuition. specialize (H1 a b). rewrite<- H9 in H11.  rewrite H_EXvis in H1; rewrite H_EXso in H1.
+                     intuition. specialize (H1 a b). rewrite<- H10 in H12.  rewrite H_EXvis in H1; rewrite H_EXso in H1.
                      auto.
 
 
             +SCase"(A a/\A b)/\(vis a b) AND a=η/\b=η'".
-                     specialize (H_soDef Ex  b a). rewrite H0 in H_soDef; rewrite H9 in H_soDef.
+                     specialize (H_soDef Ex  b a). rewrite H0 in H_soDef; rewrite H10 in H_soDef.
                      rewrite H4 in H_soDef; rewrite H_η'def in H_soDef. intuition.
-                     specialize (H1 η η'). rewrite H_EXvis in H1. rewrite H9 in H7; rewrite H0 in H7.
+                     specialize (H1 η η'). rewrite H_EXvis in H1. rewrite H10 in H8; rewrite H0 in H8.
                      auto.
 
             +SCase"(A a/\A b)/\(vis a b) AND so b a".
@@ -202,8 +206,8 @@ Proof.
   specialize (H Ex'). rewrite H_EX'vis in H; rewrite H_EX'so in H; rewrite H_EX'A in H. intuition.
   unfold WF1. rewrite  H_Exec'. intros a H_final.
   unfold not. 
-  specialize (H6 a).
-  exact H6.
+  specialize (H7 a). rewrite <- H_Exec'.
+  exact H7.
 
 Qed.
  
